A concurrency .s framework that dafny can parse

concurrency/disciplined/AppSpec.s.dfy
@@ -1,3 +1,5 @@
+include "../../lib/Lang/NativeTypes.s.dfy"
+
 // This is the application-specific part of the spec.
 // It first describes the abstract-level interface
 // (the inputs and outputs that label the transitions of a state machine),
@@ -12,6 +14,20 @@ module KeyValueType {
   type Value(==)
 
   datatype QueryResult = Found(val: Value) | NotFound
+}
+
+module MapIfc refines InputOutputIfc {
+  import opened KeyValueType
+
+  datatype Input =
+    | QueryInput(key: Key)
+    | InsertInput(key: Key, value: Value)
+    | RemoveInput(key: Key)
+
+  datatype Output =
+    | QueryOutput(res: QueryResult)
+    | InsertOutput(success: bool) // an insert may fail when there is no capacity
+    | RemoveOutput(existed: bool) // to Travis: added the possibility that there is nothing to remove
 }
 
 module MapSpec {
